test/PolyTest.v
@@ -1,0 +1,41 @@
+(*Tests for polymorphism, both in goals
+  (test monomorphization) and in hypotheses
+  (test specialization)*)
+Require Import Task.
+Require Import Theory.
+Require Import Typechecker.
+Require Import Tactics.
+From mathcomp Require Import all_ssreflect.
+Set Bullet Behavior "Strict Subproofs".
+
+(*Test 1: forall (x: 'a), x = x*)
+Module TestMonoId.
+
+Definition a : vty := vty_var "a"%string.
+Definition a' : vty := tyconst "'a".
+
+Definition x : vsymbol := ("x"%string, a).
+Definition x' : vsymbol := ("x"%string, a').
+Definition x'' := t_constsym "x" a'. 
+
+Definition id_theory : theory :=
+  [tprop Plemma "id_triv" (Fquant Tforall x (Feq a (Tvar x) (Tvar x)))].
+
+Lemma id_theory_typed : typed_theory id_theory.
+Proof.
+  check_theory.
+Qed.
+
+Ltac extra_simpl ::=
+  fold a; fold x; fold a'; fold x'; fold x''.
+
+Lemma id_theory_valid: valid_theory id_theory.
+Proof.
+  simpl. split; auto.
+  exists (["'a"%string]).
+  simpl. wstart.
+  wintros "x"%string.
+  wreflexivity.
+Qed.
+
+End TestMonoId.
